lib+spec: move definition of machine_word to Word_Lib
JIRA VER-963

lib/Word_Lib/Word_Setup_32.thy
@@ -16,16 +16,29 @@ begin
 
 text \<open>This theory defines standard platform-specific word size and alignment.\<close>
 
-definition
-  word_bits :: nat where
-  "word_bits \<equiv> len_of TYPE(32)"
+type_synonym machine_word_len = 32
+type_synonym machine_word = "machine_word_len word"
 
-definition
-  word_size :: "'a :: numeral" where
-  "word_size \<equiv> 4"
+definition word_bits :: nat
+where
+  "word_bits = len_of TYPE(machine_word_len)"
+
+text \<open>The following two are numerals so they can be used as nats and words.\<close>
+definition word_size_bits :: "'a :: numeral"
+where
+  "word_size_bits = 2"
+
+definition word_size :: "'a :: numeral"
+where
+  "word_size = 4"
 
 lemma word_bits_conv[code]:
-  "word_bits = 32" unfolding word_bits_def by simp
+  "word_bits = 32"
+  unfolding word_bits_def by simp
+
+lemma word_size_word_size_bits:
+  "(word_size::nat) = 2 ^ word_size_bits"
+  unfolding word_size_def word_size_bits_def by simp
 
 lemma word_bits_word_size_conv:
   "word_bits = word_size * 8"
